DIRTY: Add register aliasing semantics
Add basic definitions of what it means for registers to overlap or differ.

backend/IRC.ml
@@ -16,6 +16,7 @@ open AST
 open Memdata
 open Registers
 open Machregs
+open Registerfile
 open Locations
 open Conventions1
 open XTL
@@ -879,8 +880,8 @@ let record_reg_conflict cnf n =
   match (getAlias n).color with
   | Some (R r) ->
       let add_reg cnf s = Regset.add s cnf in
-      let cnf' = List.fold_left add_reg cnf (Machregs.subregs r) in
-      let cnf'' = List.fold_left add_reg cnf' (Machregs.superregs r) in
+      let cnf' = List.fold_left add_reg cnf (subreg_list r) in
+      let cnf'' = List.fold_left add_reg cnf' (superreg_list r) in
       Regset.add r cnf''
   | _ -> cnf
 
