backend/Registerfile.v
@@ -12,6 +12,7 @@
 
 Require Import OrderedType.
 Require Import Coqlib.
+Require Import Decidableplus.
 Require Import Maps.
 Require Import Ordered.
 Require Import AST.
@@ -29,6 +30,452 @@ Proof.
   destruct r; simpl; auto.
 Qed.
 
+(** * Facts about register aliasing *)
+
+(** Every architecture defines functions [subregs] and [superregs]
+  associating each register with an optional pair of subregisters and an
+  optional superregister. It must also define a type [part] and a function
+  [mreg_part] mapping subregisters of some register [r] to [PLow r] or
+  [PHigh r] as appropriate, and every "full" register [r] (that is not
+  a subregister of anything) to [PFull r].
+
+  Based on these definitions, we formulate general information about
+  register aliasing.
+
+  We define the relation [subreg r s] as meaning that [r] is strictly
+  a subregister of [s], i.e., [subreg] is irreflexive; similarly for
+  [superreg]. Registers are either the same ([mreg_eq]), non-overlapping
+  ([mreg_diff]), or overlapping ([mreg_overlap]). Registers overlap iff they
+  are in a subregister relationship.
+
+  A register's [containing_reg] is its superregister, if any; otherwise, it
+  is the register itself.
+
+  We assume that all registers are of size 32 or 64 bit. It follows that
+  a superregister is 64 bits, with exactly two 32-bit subregisters. It also
+  follows that subregisters cannot have further subregisters. *)
+
+Section REG_ALIASING.
+
+Definition subreg (r s: mreg): Prop :=
+  match subregs s with
+  | Some (lo, hi) => r = lo \/ r = hi
+  | None => False
+  end.
+
+Definition subreg_dec (r s: mreg): { subreg r s } + { ~ subreg r s }.
+Proof.
+  intros. unfold subreg. destruct (subregs s) eqn:S; auto.
+  destruct p as [lo hi]. destruct (mreg_eq r lo); auto. destruct (mreg_eq r hi); tauto.
+Defined.
+
+Lemma subreg_irrefl:
+  forall r, ~ subreg r r.
+Proof.
+  intros. destruct r; auto; unfold subreg; simpl; intuition congruence.
+Qed.
+
+Definition subreg_list r :=
+  match subregs r with
+  | Some (lo, hi) => lo :: hi :: nil
+  | None => nil
+  end.
+
+Definition superreg (r s: mreg): Prop :=
+  match superregs s with
+  | Some s => r = s
+  | None => False
+  end.
+
+Definition superreg_dec (r s: mreg): { superreg r s } + { ~ superreg r s }.
+Proof.
+  intros. unfold superreg. destruct (superregs s) eqn:S; auto.
+  destruct (mreg_eq r m); auto.
+Defined.
+
+Definition superreg_list r :=
+  match superregs r with
+  | Some s => s :: nil
+  | None => nil
+  end.
+
+Definition containing_reg (r: mreg): mreg :=
+  match superregs r with
+  | Some s => s
+  | None => r
+  end.
+
+Definition mreg_overlap (r s: mreg): Prop :=
+  subreg r s \/ subreg s r.
+
+Definition mreg_overlap_dec (r s: mreg): { mreg_overlap r s } + { ~ mreg_overlap r s }.
+Proof.
+  unfold mreg_overlap.
+  destruct (subreg_dec r s); auto.
+  destruct (subreg_dec s r); auto.
+  tauto.
+Defined.
+
+Lemma mreg_overlap_sym: forall r s, mreg_overlap r s -> mreg_overlap s r.
+Proof.
+  intros. unfold mreg_overlap in *. tauto.
+Qed.
+
+Lemma same_not_overlap:
+  forall r, ~ mreg_overlap r r.
+Proof.
+  unfold mreg_overlap, not; intros.
+  destruct H; apply subreg_irrefl in H; auto.
+Qed.
+
+Definition mreg_diff (r s: mreg): Prop :=
+  r <> s /\ ~ mreg_overlap r s.
+
+Lemma same_not_diff:
+  forall r, ~ mreg_diff r r.
+Proof.
+  unfold not, mreg_diff; intros.
+  inv H. contradict H0. reflexivity.
+Qed.
+
+Lemma not_same_not_diff_overlap:
+  forall r s, r <> s -> ~ mreg_diff r s -> mreg_overlap r s.
+Proof.
+  unfold mreg_diff; intros.
+  destruct (mreg_overlap_dec r s); auto.
+  contradict H0; auto.
+Qed.
+
+Lemma not_same_not_overlap_diff:
+  forall r s, r <> s -> ~ mreg_overlap r s -> mreg_diff r s.
+Proof.
+  unfold mreg_diff; auto.
+Qed.
+
+Lemma subreg_not_diff:
+  forall r s,
+  subreg r s ->
+  ~ mreg_diff r s.
+Proof.
+  intros. unfold mreg_diff, mreg_overlap. intuition auto.
+Qed.
+
+Lemma superreg_not_diff:
+  forall r s,
+  subreg r s ->
+  ~ mreg_diff s r.
+Proof.
+  intros. unfold mreg_diff, mreg_overlap. intuition auto.
+Qed.
+
+Lemma diff_not_eq:
+  forall r1 r2,
+  mreg_diff r1 r2 -> r1 <> r2.
+Proof.
+  unfold mreg_diff; tauto.
+Qed.
+
+Lemma diff_not_overlap:
+  forall r1 r2,
+  mreg_diff r1 r2 -> ~ mreg_overlap r1 r2.
+Proof.
+  unfold mreg_diff; tauto.
+Qed.
+
+Lemma diff_sym:
+  forall r1 r2,
+  mreg_diff r1 r2 -> mreg_diff r2 r1.
+Proof.
+  unfold mreg_diff; intros.
+  split.
+  - apply not_eq_sym. tauto.
+  - unfold not; intro. apply mreg_overlap_sym in H0. tauto.
+Qed.
+
+Definition mreg_diff_dec (r1 r2: mreg): { mreg_diff r1 r2 } + { ~ mreg_diff r1 r2 }.
+Proof.
+  unfold mreg_diff.
+  destruct (mreg_eq r1 r2); try tauto.
+  destruct (mreg_overlap_dec r1 r2); tauto.
+Defined.
+
+Lemma subreg_size:
+  forall r s,
+  subreg r s ->
+  AST.typesize (mreg_type r) = 4.
+Proof.
+  intros. destruct s; try inv H; auto.
+Qed.
+
+Lemma superreg_type:
+  forall r s,
+  subreg r s -> mreg_type s = Tany64.
+Proof.
+  intros. destruct s; try inv H; auto.
+Qed.
+
+Lemma superreg_size:
+  forall r s,
+  subreg r s ->
+  AST.typesize (mreg_type s) = 8.
+Proof.
+  intros. destruct s; try inv H; auto.
+Qed.
+
+(* Properties of the "containing" register. *)
+
+Lemma containing_reg_charact:
+  forall r, r = containing_reg r \/ subreg r (containing_reg r).
+Proof.
+  intros. destruct r; simpl; auto; unfold subreg, containing_reg; simpl; auto.
+Qed.
+
+Lemma subreg_of_containing_reg:
+  forall r s, subreg r s -> s = containing_reg r.
+Proof.
+  intros. unfold subreg, containing_reg in *.
+  destruct s; simpl in H; try tauto; destruct H; subst r; simpl; auto.
+Qed.
+
+Lemma containing_reg_idempotent:
+  forall r, containing_reg (containing_reg r) = containing_reg r.
+Proof.
+  destruct r; simpl; auto.
+Qed.
+
+Lemma overlap_containing_reg:
+  forall r s, mreg_overlap r s -> containing_reg r = containing_reg s.
+Proof.
+  intros. unfold mreg_overlap in H. destruct H as [SUB | SUB].
+  apply subreg_of_containing_reg in SUB. rewrite SUB, containing_reg_idempotent; auto.
+  apply subreg_of_containing_reg in SUB. rewrite SUB, containing_reg_idempotent; auto.
+Qed.
+
+Lemma containing_reg_diff:
+  forall r1 r2, containing_reg r1 <> containing_reg r2 -> mreg_diff r1 r2.
+Proof.
+  intros. unfold mreg_diff; split.
+  - congruence.
+  - contradict H. apply overlap_containing_reg; auto.
+Qed.
+
+(* The relationship between register parts and the other definitions. *)
+
+Lemma superreg_full:
+  forall r s,
+  subreg r s ->
+  mreg_part s = PFull s.
+Proof.
+  intros. unfold subreg in H.
+  destruct s; simpl in H; try contradiction; auto.
+Qed.
+
+Lemma subreg_low_or_high:
+  forall r s,
+  subreg r s ->
+  mreg_part r = PLow s \/ mreg_part r = PHigh s.
+Proof.
+  intros. unfold subreg in H.
+  destruct s; simpl in H; try contradiction; destruct H; subst; auto.
+Qed.
+
+Lemma subreg_cases:
+  forall r s,
+  subreg r s -> mreg_part s = PFull s /\ (mreg_part r = PLow s \/ mreg_part r = PHigh s).
+Proof.
+  intros. split; eauto using superreg_full, subreg_low_or_high.
+Qed.
+
+Lemma mreg_relation_cases:
+  forall r s,
+  r = s \/
+  (subreg r s /\ mreg_part s = PFull s /\ (mreg_part r = PLow s \/ mreg_part r = PHigh s)) \/
+  (subreg s r /\ mreg_part r = PFull r /\ (mreg_part s = PLow r \/ mreg_part s = PHigh r)) \/
+  mreg_diff r s.
+Proof.
+  intros.
+  destruct (mreg_eq r s); auto.
+  destruct (subreg_dec r s).
+    right. left. repeat split; eauto using superreg_full, subreg_low_or_high.
+  destruct (subreg_dec s r).
+    right. right. left. repeat split; eauto using superreg_full, subreg_low_or_high.
+  right. right. right. unfold mreg_diff, mreg_overlap. tauto.
+Qed.
+
+(* Relations between registers should be decidable by computation. *)
+
+Program Instance Decidable_mreg_diff: forall (x y: mreg), Decidable (mreg_diff x y) := {
+  Decidable_witness := proj_sumbool (mreg_diff_dec x y)
+}.
+Next Obligation.
+  split; intros. InvBooleans; auto. apply pred_dec_true; auto.
+Defined.
+
+Instance Finite_mreg_pair: Finite (mreg * mreg) := Finite_pair mreg mreg Finite_mreg Finite_mreg.
+
+End REG_ALIASING.
+
+(* Make it simple to apply [mreg_relation_cases]. *)
+
+Ltac compare_mregs_base do_rewrite r s :=
+  let EQ := fresh "EQ" in
+  let SUB := fresh "SUB" in
+  let FULL := fresh "FULL" in
+  let LO := fresh "LO" in
+  let HI := fresh "HI" in
+  let DIFF := fresh "DIFF" in
+  destruct (mreg_relation_cases r s) as [EQ | [[SUB [FULL [LO | HI]]] | [[SUB [FULL [LO | HI]]] | DIFF]]];
+  match do_rewrite with
+  | true =>
+    match goal with
+    | [ EQ: r = s |- _ ] =>
+      subst r; destruct (mreg_part s)
+    | _ => idtac
+    end;
+    try rewrite !FULL in *; try rewrite !LO in *; try rewrite !HI in *; auto
+  | false => idtac
+  end.
+
+Ltac compare_mregs r s := compare_mregs_base false r s.
+
+Ltac xcompare_mregs r s := compare_mregs_base true r s.
+
+(* [decide_goal] isn't powerful enough to some of the goals of the form [mreg_diff r s -> P]
+  below. This tactic helps. *)
+Ltac decide_mreg_diff_goal :=
+  refine
+    (Decidable_sound _
+      (Decidable_forall mreg Finite_mreg _
+        (fun r: mreg =>
+          Decidable_forall mreg Finite_mreg _
+            (fun s: mreg =>
+               Decidable_implies (mreg_diff r s) _
+               (Decidable_mreg_diff r s)
+               _
+            ))) _); reflexivity.
+
+Module OrderedMreg <: OrderedType.
+  Definition t := mreg.
+
+  Definition eq (x y: t) := x = y.
+  Lemma eq_refl: forall x: t, eq x x.
+  Proof (@eq_refl t).
+  Lemma eq_sym: forall x y: t, eq x y -> eq y x.
+  Proof (@eq_sym t).
+  Lemma eq_trans: forall x y z: t, eq x y -> eq y z -> eq x z.
+  Proof (@eq_trans t).
+  Definition eq_dec := mreg_eq.
+
+  Open Scope positive_scope.
+
+  Definition lt (x y: t) :=
+    IndexedMreg.index x < IndexedMreg.index y.
+
+  Lemma lt_trans: forall x y z: t, lt x y -> lt y z -> lt x z.
+  Proof.
+    intros. eapply Pos.lt_trans; eauto.
+  Qed.
+
+  Lemma lt_not_eq: forall x y: t, lt x y -> x <> y.
+  Proof.
+    intros. apply Plt_ne in H. contradict H; congruence.
+  Qed.
+
+  Lemma compare: forall x y: t, Compare lt eq x y.
+  Proof.
+    intros. destruct (OrderedPositive.compare (IndexedMreg.index x) (IndexedMreg.index y)).
+    - apply LT. red. auto.
+    - apply EQ. red. auto using IndexedMreg.index_inj.
+    - apply GT. red. auto.
+  Qed.
+
+  Instance Decidable_lt (x y: t): Decidable (lt x y) :=
+    Decidable_lt_positive (IndexedMreg.index x) (IndexedMreg.index y).
+
+  (** Define intervals of registers as follows:
+      - A register [R] that is not involved in register pairing maps to the
+        interval [(R, R)], i.e., it is its own upper and lower bound.
+      - A paired register [D = S_low:S_high] maps to the interval
+        [(S_low, S_high)]. Its two component registers map to the intervals
+        [(S_low, D)] and [(D, S_high)], respectively.
+      The [Machregs] module must define [diff_low_bound] and [diff_high_bound]
+      functions conforming to this specification.
+   *)
+
+  Lemma low_bound_lt_or_eq: forall r: t, lt (diff_low_bound r) r \/ diff_low_bound r = r.
+  Proof.
+    intros. destruct r; compute; try tauto.
+  Qed.
+
+  Lemma lt_low_bound_not_subreg:
+    forall r p, lt p (diff_low_bound r) -> ~ subreg r p.
+  Proof.
+    intros.
+    destruct p; compute; auto;
+      intros; decompose [or] H0; subst; compute in H; congruence.
+  Qed.
+
+  Lemma lt_low_bound_not_subreg':
+    forall r p, lt p (diff_low_bound r) -> ~ subreg p r.
+  Proof.
+    intros.
+    destruct r; compute; auto;
+      intros; decompose [or] H0; subst; compute in H; congruence.
+  Qed.
+
+  Lemma lt_or_eq_high_bound: forall r: t, lt r (diff_high_bound r) \/ r = diff_high_bound r.
+  Proof.
+    intros. destruct r; compute; tauto.
+  Qed.
+
+  Lemma high_bound_lt_not_subreg:
+    forall r p, lt (diff_high_bound r) p -> ~ subreg r p.
+  Proof.
+    intros.
+    destruct p; compute; auto;
+      intros; decompose [or] H0; subst; compute in H; congruence.
+  Qed.
+
+  Lemma high_bound_lt_not_subreg':
+    forall r p, lt (diff_high_bound r) p -> ~ subreg p r.
+  Proof.
+    intros.
+    destruct r; compute; auto;
+      intros; decompose [or] H0; subst; compute in H; congruence.
+  Qed.
+
+  Definition diff_low_bound r := Machregs.diff_low_bound r.
+  Definition diff_high_bound r := Machregs.diff_high_bound r.
+
+  Lemma outside_interval_diff:
+    forall r r', lt r' (diff_low_bound r) \/ lt (diff_high_bound r) r' -> mreg_diff r r'.
+  Proof.
+    unfold diff_low_bound, diff_high_bound. intros r r' [A | B].
+    - split.
+      + generalize (low_bound_lt_or_eq r); intros [C | D].
+        * eapply not_eq_sym, lt_not_eq, lt_trans; eauto.
+        * rewrite D in A. apply not_eq_sym, lt_not_eq; auto.
+      + generalize (lt_low_bound_not_subreg r r' A); intros.
+        generalize (lt_low_bound_not_subreg' r r' A); intros.
+        unfold mreg_overlap. intuition auto.
+    - split.
+      + generalize (lt_or_eq_high_bound r); intros [C | D].
+        * eapply lt_not_eq, lt_trans; eauto.
+        * rewrite <- D in B. apply lt_not_eq; auto.
+      + generalize (high_bound_lt_not_subreg r r' B); intros.
+        generalize (high_bound_lt_not_subreg' r r' B); intros.
+        unfold mreg_overlap. intuition auto.
+  Qed.
+
+  Lemma diff_outside_interval:
+    forall r r',
+    mreg_diff r r' -> lt r' (diff_low_bound r) \/ lt (diff_high_bound r) r'.
+  Proof.
+    decide_mreg_diff_goal.
+  Qed.
+
+End OrderedMreg.
+
 (** * Representation of the register file *)
 
 (** The [Regfile] module defines mappings from registers to values. The register
@@ -45,18 +492,24 @@ Module Regfile.
   Definition init := ZMap.init Undef.
 
   (* A register's address: The index of its first byte. *)
-  Definition addr (r: mreg) : Z := Zpos (IndexedMreg.index r) * 4.
+  Definition addr (r: mreg) : Z :=
+    let base_addr reg := Zpos (IndexedMreg.index reg) * 4 in
+    match mreg_part r with
+      | PFull r => base_addr r
+      | PLow s  => base_addr s
+      | PHigh s => base_addr s + 4
+    end.
 
   Remark addr_pos: forall r, addr r > 0.
   Proof.
-    intros. unfold addr. xomega.
+    intros. unfold addr. destruct (mreg_part r); xomega.
   Qed.
 
   (* The address one byte past the end of register [r]. The next nonoverlapping
      register may start here. *)
   Definition next_addr (r: mreg) : Z := addr r + AST.typesize (mreg_type r).
 
-  Lemma outside_interval_diff:
+  Lemma outside_interval_neq:
     forall r s, next_addr r <= addr s \/ next_addr s <= addr r -> r <> s.
   Proof.
     intros. destruct H; unfold next_addr in H.
@@ -64,16 +517,35 @@ Module Regfile.
     generalize (AST.typesize_pos (mreg_type s)); intros. contradict H. subst. omega.
   Qed.
 
+  Lemma outside_interval_diff:
+    forall r s, next_addr r <= addr s \/ next_addr s <= addr r -> mreg_diff r s.
+  Proof.
+    intros. destruct H; unfold next_addr, addr in H.
+    generalize (AST.typesize_pos (mreg_type r)); intros.
+    xcompare_mregs r s; try omega.
+    apply superreg_size in SUB; omega.
+    generalize (AST.typesize_pos (mreg_type s)); intros.
+    xcompare_mregs s r; try omega.
+    apply superreg_size in SUB; omega.
+    auto using diff_sym.
+  Qed.
+
   Lemma address_lt:
     forall r s,
-    r <> s ->
+    mreg_diff r s ->
     addr r < addr s ->
     next_addr r <= addr s.
   Proof.
-    intros. unfold addr in H0.
-    apply IndexedMreg.scaled_index_with_size; omega.
+    decide_mreg_diff_goal.
   Qed.
 
+  Lemma diff_outside_interval:
+    forall r s, mreg_diff r s -> next_addr r <= addr s \/ next_addr s <= addr r.
+  Proof.
+    decide_mreg_diff_goal.
+  Qed.
+
+  (*
   Lemma diff_outside_interval:
     forall r s, r <> s -> next_addr r <= addr s \/ next_addr s <= addr r.
   Proof.
@@ -85,6 +557,7 @@ Module Regfile.
     - left. apply address_lt; auto.
     - right. apply address_lt; auto.
   Qed.
+*)
 
   Definition chunk_of_mreg (r: mreg) : memory_chunk :=
     chunk_of_type (mreg_type r).
@@ -135,7 +608,7 @@ Module Regfile.
 
   Lemma gso:
     forall r s v rf,
-    r <> s ->
+    mreg_diff r s ->
     get r (set s v rf) = get r rf.
   Proof.
     intros. unfold get, set, get_bytes, set_bytes.
@@ -146,6 +619,276 @@ Module Regfile.
     rewrite !Z2Nat.id; omega.
   Qed.
 
+  (*
+  Lemma gu_subreg:
+    forall r s rf,
+    subreg r s ->
+    get r (set s Vundef rf) = Vundef.
+  Proof.
+    intros. unfold get, set, get_bytes, set_bytes, addr.
+    generalize (subreg_cases r s H); intros [FULL [LO | HI]]; rewrite FULL.
+    - rewrite LO.
+      unfold chunk_of_mreg.
+      rewrite (subreg_size r s H), (superreg_type r s H).
+      rewrite Mem.getN_setN_prefix.
+      destruct (chunk_of_type (mreg_type r)); simpl; auto.
+      simpl; auto.
+    - rewrite HI.
+      unfold chunk_of_mreg.
+      rewrite (subreg_size r s H), (superreg_type r s H).
+      replace 4 with (Z.of_nat (Z.to_nat 4)) at 3; auto.
+      rewrite Mem.getN_setN_suffix.
+      destruct (chunk_of_type (mreg_type r)); simpl; auto.
+      simpl; auto.
+  Qed.
+*)
+
+  Lemma gu_subreg:
+    forall r s v rf,
+    subreg r s ->
+    get r (set s v rf) = Vundef.
+  Proof.
+    intros. unfold get, set, get_bytes, set_bytes, addr.
+    generalize (subreg_cases r s H); intros [FULL [LO | HI]]; rewrite FULL.
+    - rewrite LO.
+      unfold chunk_of_mreg.
+      rewrite (subreg_size r s H), (superreg_type r s H).
+      rewrite Mem.getN_setN_prefix.
+
+      destruct (chunk_of_type (mreg_type r)); simpl; auto; destruct v; simpl; auto;
+      unfold decode_val, proj_bytes; destruct Archi.ptr64; simpl; auto; rewrite !andb_false_r; simpl; auto.
+
+      destruct v; simpl; auto.
+    - rewrite HI.
+      unfold chunk_of_mreg.
+      rewrite (subreg_size r s H), (superreg_type r s H).
+      replace 4 with (Z.of_nat (Z.to_nat 4)) at 3; auto.
+      rewrite Mem.getN_setN_suffix.
+
+      destruct (chunk_of_type (mreg_type r)); simpl; auto; destruct v; simpl; auto;
+      unfold decode_val, proj_bytes; destruct Archi.ptr64; simpl; auto; rewrite !andb_false_r; simpl; auto.
+
+      destruct v; simpl; auto.
+  Qed.
+
+  Lemma decode_undef_suffix:
+    forall a b c d,
+    decode_val Many64 (a :: b :: c :: d :: Undef :: Undef :: Undef :: Undef :: nil) = Vundef.
+  Proof.
+    intros.
+    set (undefs := Undef :: Undef :: Undef :: Undef :: nil).
+    change (a :: b :: c :: d :: undefs) with ((a :: b :: c :: d :: nil) ++ undefs).
+    unfold decode_val. rewrite proj_bytes_append.
+    simpl (proj_bytes undefs).
+    destruct a, b, c, d; simpl; auto; rewrite !andb_false_r; auto.
+  Qed.
+
+  Lemma gu_superreg':
+    forall r s rf,
+    subreg r s ->
+    get s (set r Vundef rf) = Vundef.
+  Proof.
+    intros. unfold get, set, get_bytes, set_bytes, addr.
+    generalize (subreg_cases r s H); intros [FULL [LO | HI]]; rewrite FULL.
+    - rewrite LO.
+      unfold chunk_of_mreg.
+      rewrite (superreg_type r s H).
+      simpl typesize.
+      change (Z.to_nat 8) with (4 + 4)%nat.
+      rewrite Mem.getN_concat.
+      simpl chunk_of_type.
+      replace (4%nat) with (length (encode_val (chunk_of_type (mreg_type r)) Vundef)).
+      rewrite Mem.getN_setN_same.
+      rewrite Mem.getN_setN_outside.
+      destruct (mreg_type r); simpl; unfold decode_val; simpl; auto.
+      omega.
+      apply subreg_size in H.
+      destruct (mreg_type r); simpl; auto; inv H.
+    - rewrite HI.
+      unfold chunk_of_mreg.
+      rewrite (superreg_type r s H).
+      simpl typesize.
+      change (Z.to_nat 8) with (4 + 4)%nat.
+      rewrite Mem.getN_concat.
+      simpl chunk_of_type.
+      rewrite Mem.getN_setN_outside.
+
+      replace (Z.pos (IndexedMreg.index s) * 4 + Z.of_nat 4) with (addr r).
+      replace (Z.pos (IndexedMreg.index s) * 4 + 4) with (addr r).
+      replace (4%nat) with (length (encode_val (chunk_of_type (mreg_type r)) Vundef)).
+      rewrite Mem.getN_setN_same.
+      apply subreg_size in H.
+      destruct (mreg_type r); try inv H; simpl encode_val. try apply decode_undef_suffix.
+      apply decode_undef_suffix.
+      unfold decode_val.
+
+      erewrite proj_value_diff_q with (q := Q32).
+      simpl Val.load_result.
+      destruct (proj_bytes _); auto.
+      congruence.
+      apply in_app. right. unfold inj_value. simpl inj_value_rec. eapply in_eq.
+
+      apply subreg_size in H.
+      destruct (mreg_type r); simpl; try inv H; auto.
+      unfold addr. rewrite HI; congruence.
+      unfold addr. rewrite HI. f_equal.
+      left.
+      simpl. omega.
+  Qed.
+
+  Lemma gu_superreg:
+    forall r s v rf,
+    subreg r s ->
+    get s (set r v rf) = Vundef.
+  Proof.
+    intros. unfold get, set, get_bytes, set_bytes, addr.
+    generalize (subreg_cases r s H); intros [FULL [LO | HI]]; rewrite FULL.
+    - rewrite LO.
+      unfold chunk_of_mreg.
+      rewrite (superreg_type r s H).
+      simpl typesize.
+      change (Z.to_nat 8) with (4 + 4)%nat.
+      rewrite Mem.getN_concat.
+      simpl chunk_of_type.
+      replace (4%nat) with (length (encode_val (chunk_of_type (mreg_type r)) v)).
+      rewrite Mem.getN_setN_same.
+      rewrite Mem.getN_setN_outside.
+
+      unfold decode_val.
+      replace (length (encode_val (chunk_of_type (mreg_type r)) v)) with 4%nat.
+      apply subreg_size in H.
+      destruct (mreg_type r); try inv H.
+
+      destruct v; simpl; auto.
+      rewrite proj_value_encode_int_app_l; auto.
+      destruct (proj_bytes _); auto.
+      destruct Archi.ptr64. simpl proj_value. destruct (proj_bytes _); auto.
+      unfold inj_value. simpl inj_value_rec.
+      erewrite proj_value_diff_q with (q := Q32).
+      destruct (proj_bytes _); auto.
+      congruence.
+      apply in_app. left. eapply in_eq.
+
+      destruct v; simpl; auto.
+      rewrite proj_value_encode_int_app_l; auto.
+      destruct (proj_bytes _); auto.
+
+      destruct v; simpl; rewrite !andb_false_r; auto.
+      apply subreg_size in H.
+      destruct (mreg_type r); simpl; try inv H; auto.
+      destruct v; simpl; auto.
+      rewrite length_inj_bytes, encode_int_length; auto.
+      destruct v; simpl; auto.
+      rewrite length_inj_bytes, encode_int_length; auto.
+      destruct v; simpl; auto.
+      omega.
+      apply subreg_size in H.
+      destruct (mreg_type r); simpl; try inv H; auto.
+      destruct v; simpl; auto.
+      rewrite length_inj_bytes, encode_int_length; auto.
+      destruct v; simpl; auto.
+      rewrite length_inj_bytes, encode_int_length; auto.
+      destruct v; simpl; auto.
+
+    - rewrite HI.
+      unfold chunk_of_mreg.
+      rewrite (superreg_type r s H).
+      simpl typesize.
+      change (Z.to_nat 8) with (4 + 4)%nat.
+      rewrite Mem.getN_concat.
+      simpl chunk_of_type.
+      rewrite Mem.getN_setN_outside.
+
+      replace (Z.pos (IndexedMreg.index s) * 4 + Z.of_nat 4) with (addr r).
+      replace (Z.pos (IndexedMreg.index s) * 4 + 4) with (addr r).
+      replace (4%nat) with (length (encode_val (chunk_of_type (mreg_type r)) v)).
+      rewrite Mem.getN_setN_same.
+      apply subreg_size in H.
+      destruct (mreg_type r); try inversion H; simpl encode_val.
+
+      unfold decode_val.
+      destruct v; simpl encode_val; try apply decode_undef_suffix.
+      rewrite proj_value_encode_int_app_r. destruct (proj_bytes _); auto. auto.
+
+      destruct Archi.ptr64. apply decode_undef_suffix.
+      unfold inj_value. simpl inj_value_rec.
+      erewrite proj_value_diff_q with (q := Q32).
+      destruct (proj_bytes _); auto.
+      congruence.
+      apply in_app. right. eapply in_eq.
+
+      destruct v; simpl; try apply decode_undef_suffix.
+      unfold decode_val.
+      rewrite proj_value_encode_int_app_r. destruct (proj_bytes _); auto. auto.
+
+      unfold decode_val.
+      erewrite proj_value_diff_q with (q := Q32).
+      destruct (proj_bytes _); auto.
+      congruence.
+      apply in_app. right. destruct v; simpl; auto.
+
+      apply subreg_size in H.
+      destruct (mreg_type r); simpl; try inv H; auto.
+      destruct v; simpl; auto.
+      rewrite length_inj_bytes, encode_int_length; auto.
+      destruct v; simpl; auto.
+      rewrite length_inj_bytes, encode_int_length; auto.
+      destruct v; simpl; auto.
+
+      unfold addr. rewrite HI; congruence.
+      unfold addr. rewrite HI. f_equal.
+      left.
+      simpl. omega.
+  Qed.
+
+  Lemma gu_overlap':
+    forall r s rf,
+    mreg_overlap r s ->
+    get r (set s Vundef rf) = Vundef.
+  Proof.
+    intros.
+    xcompare_mregs r s.
+    - rewrite gss; destruct (chunk_of_mreg s); auto.
+    - rewrite gss; destruct (chunk_of_mreg s); auto.
+    - rewrite gss; destruct (chunk_of_mreg s); auto.
+    - unfold get, set. unfold get_bytes, set_bytes. unfold addr.
+      rewrite LO, FULL.
+      unfold chunk_of_mreg.
+      rewrite (subreg_size r s SUB), (superreg_type r s SUB).
+      rewrite Mem.getN_setN_prefix.
+      simpl. destruct (chunk_of_type (mreg_type r)); simpl; auto.
+      simpl. auto.
+    - unfold get, set. unfold get_bytes, set_bytes. unfold addr.
+      rewrite HI, FULL.
+      unfold chunk_of_mreg.
+      rewrite (subreg_size r s SUB), (superreg_type r s SUB).
+      replace 4 with (Z.of_nat (Z.to_nat 4)) at 3; auto.
+      rewrite Mem.getN_setN_suffix.
+      simpl. destruct (chunk_of_type (mreg_type r)); simpl; auto.
+      simpl. auto.
+    - apply gu_superreg; auto.
+    - apply gu_superreg; auto.
+    - apply diff_not_overlap in DIFF; tauto.
+  Qed.
+
+  Lemma gu_overlap:
+    forall r s v rf,
+    mreg_overlap r s ->
+    get r (set s v rf) = Vundef.
+  Proof.
+    intros.
+    xcompare_mregs r s.
+    - apply same_not_overlap in H; tauto.
+    - apply same_not_overlap in H; tauto.
+    - apply same_not_overlap in H; tauto.
+    - apply gu_subreg; auto.
+    - apply gu_subreg; auto.
+    - apply gu_superreg; auto.
+    - apply gu_superreg; auto.
+    - apply diff_not_overlap in DIFF; tauto.
+  Qed.
+
+  (*
   Lemma override_in:
     forall rs r new old,
     In r rs -> get r (override rs new old) = get r new.
@@ -167,5 +910,6 @@ Module Regfile.
     intros. induction rs; auto.
     apply not_in_cons in H. simpl. rewrite gso; intuition auto.
   Qed.
+*)
 
 End Regfile.
